

Velocity of Screw Motion

To find the velocity of screw motion without differentiation, consider the homogeneous transformation:

$$\mathbf{g}_{ab}(\theta) = e^{\hat{\xi}\theta} \mathbf{g}_{ab}(0)$$

Taking the derivative of the above, we find:

$$\dot{\mathbf{g}}_{ab}(\theta) = \frac{d}{dt} \left(e^{\hat{\xi}\theta} \right) \mathbf{g}_{ab}(0) = \hat{\xi} \dot{\theta} e^{\hat{\xi}\theta} \mathbf{g}_{ab}(0)$$

We can use this expression in the equation for spatial velocity:

$$\begin{aligned} \hat{\mathbf{V}}_{ab}^s &= \dot{\mathbf{g}}_{ab}(\theta) \mathbf{g}_{ab}^{-1}(\theta) \\ \hat{\mathbf{V}}_{ab}^s &= \hat{\xi} \dot{\theta} e^{\hat{\xi}\theta} \mathbf{g}_{ab}(0) \mathbf{g}_{ab}^{-1}(\theta) & \because \quad \dot{\mathbf{g}}_{ab}(\theta) &= \hat{\xi} \dot{\theta} e^{\hat{\xi}\theta} \mathbf{g}_{ab}(0) \\ \hat{\mathbf{V}}_{ab}^s &= \hat{\xi} \dot{\theta} e^{\hat{\xi}\theta} \underbrace{\mathbf{g}_{ab}(0) \mathbf{g}_{ab}^{-1}(0)}_{\mathbf{I}} e^{-\hat{\xi}\theta} & \because \quad \mathbf{g}_{ab}^{-1}(\theta) &= \left(e^{\hat{\xi}\theta} \mathbf{g}_{ab}(0) \right)^{-1} = \mathbf{g}_{ab}^{-1}(0) e^{-\hat{\xi}\theta} \\ \hat{\mathbf{V}}_{ab}^s &= \hat{\xi} \dot{\theta} \underbrace{e^{\hat{\xi}\theta} e^{-\hat{\xi}\theta}}_{\mathbf{I}} \\ \boxed{\hat{\mathbf{V}}_{ab}^s} &= \boxed{\hat{\xi} \dot{\theta}} \end{aligned}$$



Velocity of Screw Motion

Body velocity can be found in a similar fashion:

$$\hat{\mathbf{V}}_{ab}^b = \mathbf{g}_{ab}^{-1}(\theta) \dot{\mathbf{g}}_{ab}(\theta)$$

$$\hat{\mathbf{V}}_{ab}^b = \mathbf{g}_{ab}^{-1}(0) e^{-\hat{\xi}\theta} \dot{\mathbf{g}}_{ab}(\theta) \quad \because \quad \mathbf{g}_{ab}^{-1}(\theta) = \mathbf{g}_{ab}^{-1}(0) e^{-\hat{\xi}\theta}$$

$$\hat{\mathbf{V}}_{ab}^b = \mathbf{g}_{ab}^{-1}(0) e^{-\hat{\xi}\theta} \hat{\xi} \dot{\theta} e^{\hat{\xi}\theta} \mathbf{g}_{ab}(0) \quad \because \quad \dot{\mathbf{g}}_{ab}(\theta) = \hat{\xi} \dot{\theta} e^{\hat{\xi}\theta} \mathbf{g}_{ab}(0)$$

$$\hat{\mathbf{V}}_{ab}^b = \mathbf{g}_{ab}^{-1}(0) \left(e^{-\hat{\xi}\theta} \hat{\xi} e^{\hat{\xi}\theta} \right) \mathbf{g}_{ab}(0) \dot{\theta}$$

$$\hat{\mathbf{V}}_{ab}^b = \mathbf{g}_{ab}^{-1}(0) \hat{\xi} \mathbf{g}_{ab}(0) \dot{\theta} \quad \because \quad e^{-\hat{\xi}\theta} \hat{\xi} e^{\hat{\xi}\theta} = \hat{\xi}$$

$$\boxed{\hat{\mathbf{V}}_{ab}^b = \left(\text{Ad}_{\mathbf{g}_{ab}^{-1}(0)} \hat{\xi} \right)^\wedge \dot{\theta}}$$

